add the 'and' opperation for words too

TCB/BinaryProps.v
@@ -21,7 +21,7 @@ Proof.
   repeat rewrite fst_four_bits_of_half_byte. reflexivity.
 Qed.
 
-Lemma fst_word_of_word: forall w,
+Lemma word_of_word: forall w,
   to_word (word_to_N w) = w.
 Proof.
   destruct w as [b1 b2 b3 b4].
@@ -30,4 +30,12 @@ Proof.
   unfold fst_byte, byte_to_N.
   rewrite fst_four_bits_of_half_byte.
   destruct b4. simpl. destruct h; reflexivity.
+Qed.
+
+Definition word_and w1 w2 :=
+  to_word (N_and (word_to_N w1) (word_to_N w2)).
+
+Lemma word_and_same w: word_and w w = w.
+Proof.
+  unfold word_and. rewrite N_and_same. apply word_of_word.
 Qed.
